Add comments to WfReflective, handle Expr
In addition to much better documentation in WfReflective, we now also have a
single tactic that handles goals of [Wf], on [Expr].

src/Reflection/WfReflective.v
@@ -1,47 +1,85 @@
+(** * A reflective Version of [Wf] proofs *)
+(** Because every constructor of [Syntax.wff] stores the syntax tree
+    being proven well-formed, a proof that a syntax tree is
+    well-formed is quadratic in the size of the syntax tree.  (Tacking
+    an extra term on to the head of the syntax tree requires an extra
+    constructor of [Syntax.wff], and that constructor stores the
+    entirety of the new syntax tree.)
+
+    In practice, this makes proving well-formedness of large trees
+    very slow.  To remedy this, we provide an alternative type
+    ([reflect_wffT]) that implies [Syntax.wff], but is only linear in
+    the size of the syntax tree, with a coefficient less than 1.
+
+    The idea is that, since we already know the syntax-tree arguments
+    to the constructors (and, moreover, already fully know the shape
+    of the [Syntax.wff] proof, because it will exactly match the shape
+    of the syntax tree), the proof doesn't have to store any of that
+    information.  It only has to store the genuinely new information
+    in [Syntax.wff], namely, that the constants don't depend on the
+    [var] argument (i.e., that the constants in the same location in
+    the two expressions are equal), and that there are no free nor
+    mismatched variables (i.e., that the variables in the same
+    location in the two expressions are in the relevant list of
+    binders).  We can make the further optimization of storing the
+    location in the list of each binder, so that all that's left to
+    verify is that the locations line up correctly.
+
+    Since there is no way to assign list locations (De Bruijn indices)
+    after the fact (that is, once we have an [exprf var t] rather than
+    an [Expr t]), we instead start from an expression where [var] is
+    enriched with De Bruijn indices, and talk about [Syntax.wff] of
+    that expression stripped of its De Bruijn indices.  Since this
+    procedure is only expected to work on concrete syntax trees, we
+    will be able to simply check by unification to check that
+    stripping the indices results in the term that we started with.
+
+    The interface of this file is that, to prove a [Syntax.Wf] goal,
+    you invoke the tactic [reflect_Wf base_type_eq_semidec_is_dec
+    op_beq_bl], where:
+
+    - [base_type_eq_semidec_is_dec : forall t1 t2,
+       base_type_eq_semidec_transparent t1 t2 = None -> t1 <> t2] for
+       some [base_type_eq_semidec_transparent : forall t1 t2 :
+       base_type_code, option (t1 = t2)], and
+
+    - [op_beq_bl : forall t1 tR x y, prop_of_option (op_beq t1 tR x y)
+      -> x = y] for some [op_beq : forall t1 tR, op t1 tR -> op t1 tR
+      -> option pointed_Prop] *)
+
 Require Import Coq.Arith.Arith Coq.Logic.Eqdep_dec.
 Require Import Crypto.Reflection.Syntax.
-Require Import Crypto.Util.Notations Crypto.Util.Tactics Crypto.Util.Option Crypto.Util.Sigma Crypto.Util.Prod.
+Require Import Crypto.Util.Notations Crypto.Util.Tactics Crypto.Util.Option Crypto.Util.Sigma Crypto.Util.Prod Crypto.Util.Decidable.
+Require Export Crypto.Util.PointedProp. (* export for the [bool >-> option pointed_Prop] coercion *)
+Require Export Crypto.Util.FixCoqMistakes.
 
-Inductive pointed_Prop := trivial | inject (_ : Prop).
-Definition and_pointed_Prop (x y : pointed_Prop) : pointed_Prop
-  := match x, y with
-     | trivial, trivial => trivial
-     | trivial, inject p => inject p
-     | inject p, trivial => inject p
-     | inject p, inject q => inject (p /\ q)
-     end.
-Definition to_prop (x : pointed_Prop) : Prop
-  := match x with
-     | trivial => True
-     | inject p => p
-     end.
-
-Local Infix "/\" := and_pointed_Prop : type_scope.
-
-Definition f_equal2 {A1 A2 B} (f : A1 -> A2 -> B) {x1 y1 : A1} {x2 y2 : A2} (H : x1 = y1)
-  := match H in (_ = y) return (x2 = y2 -> f x1 x2 = f y y2) with
-     | eq_refl =>
-       fun H0 : x2 = y2 =>
-         match H0 in (_ = y) return (f x1 x2 = f x1 y) with
-         | eq_refl => eq_refl
-         end
-     end.
 
 Section language.
+  (** To be able to optimize away so much of the [Syntax.wff] proof,
+      we must be able to decide a few things: equality of base types,
+      and equality of operator codes.  Since we will be casting across
+      the equality proofs of base types, we require that this
+      semi-decider give transparent proofs.  (This requirement is not
+      enforced, but it will block [vm_compute] when trying to use the
+      lemma in this file.) *)
   Context (base_type_code : Type).
   Context (interp_base_type : base_type_code -> Type).
   Context (base_type_eq_semidec_transparent : forall t1 t2 : base_type_code, option (t1 = t2)).
   Context (base_type_eq_semidec_is_dec : forall t1 t2, base_type_eq_semidec_transparent t1 t2 = None -> t1 <> t2).
   Context (op : flat_type base_type_code -> flat_type base_type_code -> Type).
+  (** In practice, semi-deciding equality of operators should either
+      return [Some trivial] or [None], and not make use of the
+      generality of [pointed_Prop].  However, we need to use
+      [pointed_Prop] internally because we need to talk about equality
+      of things of type [var t], for [var : base_type_code -> Type].
+      It does not hurt to allow extra generality in [op_beq]. *)
   Context (op_beq : forall t1 tR, op t1 tR -> op t1 tR -> option pointed_Prop).
-  Context (op_beq_bl : forall t1 tR x y, match op_beq t1 tR x y with
-                                    | Some p => to_prop p
-                                    | _ => False
-                                    end -> x = y).
+  Context (op_beq_bl : forall t1 tR x y, prop_of_option (op_beq t1 tR x y) -> x = y).
   Context {var1 var2 : base_type_code -> Type}.
 
   Local Notation eP := (fun t => var1 (fst t) * var2 (snd t))%type (only parsing).
 
+  (* convenience notations that fill in some arguments used across the section *)
   Local Notation flat_type := (flat_type base_type_code).
   Local Notation type := (type base_type_code).
   Let Tbase := @Tbase base_type_code.
@@ -49,21 +87,17 @@ Section language.
   Local Notation interp_type := (interp_type interp_base_type).
   Local Notation interp_flat_type := (interp_flat_type_gen interp_base_type).
   Local Notation exprf := (@exprf base_type_code interp_base_type op).
+  Local Notation expr := (@expr base_type_code interp_base_type op).
 
-  (*Fixpoint eq_interp_flat_type (t1 t2 : flat_type)
-    : interp_flat_type t1 -> interp_flat_type t2 -> option pointed_Prop
-    := match t1, t2 return interp_flat_type t1 -> interp_flat_type t2 -> option _ with
-       | Prod A B, Prod A' B'
-         => fun x y => match @eq_interp_flat_type A A' (fst x) (fst y),
-                         @eq_interp_flat_type B B' (snd x) (snd y) with
-                   | Some p, Some q => Some (p /\ q)
-                   | _, _ => None
-                   end
-       | Prod _ _, _ => fun _ _ => None
-       | Syntax.Tbase t1, Syntax.Tbase t2
-         => fun x y => base_type_eq_and_cast t1 t2 x y (*Some (exists pf : t1 = t2, eq_rect _ interp_base_type x _ pf = y)*)
-       | Syntax.Tbase _, _ => fun _ _ => None
-       end.*)
+  Local Ltac inversion_base_type_code_step :=
+    match goal with
+    | [ H : ?x = ?x :> base_type_code |- _ ]
+      => assert (H = eq_refl) by eapply UIP_dec, dec_rel_of_semidec_rel, base_type_eq_semidec_is_dec; subst H
+    | [ H : ?x = ?y :> base_type_code |- _ ] => subst x || subst y
+    end.
+  Local Ltac inversion_base_type_code := repeat inversion_base_type_code_step.
+
+  (* lift [base_type_eq_semidec_transparent] across [flat_type] *)
   Fixpoint flat_type_eq_semidec_transparent (t1 t2 : flat_type) : option (t1 = t2)
     := match t1, t2 return option (t1 = t2) with
        | Syntax.Tbase t1, Syntax.Tbase t2
@@ -77,6 +111,41 @@ Section language.
            end
        | Prod _ _, _ => None
        end.
+  Fixpoint type_eq_semidec_transparent (t1 t2 : type) : option (t1 = t2)
+    := match t1, t2 return option (t1 = t2) with
+       | Syntax.Tflat t1, Syntax.Tflat t2
+         => option_map (@f_equal _ _ (@Tflat _) _ _)
+                      (flat_type_eq_semidec_transparent t1 t2)
+       | Syntax.Tflat _, _ => None
+       | Arrow A B, Arrow A' B'
+         => match base_type_eq_semidec_transparent A A', type_eq_semidec_transparent B B' with
+           | Some p, Some q => Some (f_equal2 (@Arrow base_type_code) p q)
+           | _, _ => None
+           end
+       | Arrow _ _, _ => None
+       end.
+  Lemma base_type_eq_semidec_transparent_refl t : base_type_eq_semidec_transparent t t = Some eq_refl.
+  Proof.
+    clear -base_type_eq_semidec_is_dec.
+    pose proof (base_type_eq_semidec_is_dec t t).
+    destruct (base_type_eq_semidec_transparent t t); intros; try intuition congruence.
+    inversion_base_type_code; reflexivity.
+  Qed.
+  Lemma flat_type_eq_semidec_transparent_refl t : flat_type_eq_semidec_transparent t t = Some eq_refl.
+  Proof.
+    clear -base_type_eq_semidec_is_dec.
+    induction t as [t | A B IHt]; simpl.
+    { rewrite base_type_eq_semidec_transparent_refl; reflexivity. }
+    { rewrite_hyp !*; reflexivity. }
+  Qed.
+  Lemma type_eq_semidec_transparent_refl t : type_eq_semidec_transparent t t = Some eq_refl.
+  Proof.
+    clear -base_type_eq_semidec_is_dec.
+    induction t as [t | A B IHt]; simpl.
+    { rewrite flat_type_eq_semidec_transparent_refl; reflexivity. }
+    { rewrite base_type_eq_semidec_transparent_refl; rewrite_hyp !*; reflexivity. }
+  Qed.
+
   Definition op_beq' t1 tR t1' tR' (x : op t1 tR) (y : op t1' tR') : option pointed_Prop
     := match flat_type_eq_semidec_transparent t1 t1', flat_type_eq_semidec_transparent tR tR' with
        | Some p, Some q
@@ -86,16 +155,44 @@ Section language.
        | _, _ => None
        end.
 
-  Definition eq_type_and_var : sigT eP -> sigT eP -> option pointed_Prop
-    := fun x y =>
-         let 'existT (t1, t2) (a, b) := x in
-         let 'existT (t1', t2') (a', b') := y in
-         match base_type_eq_semidec_transparent t1 t1', base_type_eq_semidec_transparent t2 t2' with
-         | Some p, Some q
-           => Some (inject (and (eq_rect _ var1 a _ p = a') (eq_rect _ var2 b _ q = b')))
-         | _, _ => None
-         end.
+  (** While [Syntax.wff] is parameterized over a list of [sigT (fun t
+      => var1 t * var2 t)], it is simpler here to make everything
+      heterogenous, rather than trying to mix homogenous and
+      heterogenous things.† Thus we parameterize our [reflect_wffT]
+      over a list of [sigT (fun t => var1 (fst t) * var2 (snd t))],
+      and write a function ([duplicate_type]) that turns the former
+      into the latter.
 
+      † This is an instance of the general theme that abstraction
+        barriers are important.  Here we enforce the abstraction
+        barrier that our input decision procedures are homogenous, but
+        all of our internal code is strictly heterogenous.  This
+        allows us to contain the conversions between homogenous and
+        heterogenous code to a few functions: [op_beq'],
+        [eq_type_and_var], [eq_type_and_const], and to the statement
+        about [Syntax.wff] itself.  *)
+
+  Definition eq_semidec_and_gen {T} (semidec : forall x y : T, option (x = y))
+             (t t' : T) (f : T -> Type) (x : f t) (x' : f t')
+    : option pointed_Prop
+    := match semidec t t' with
+       | Some p
+         => Some (inject (eq_rect _ f x _ p = x'))
+       | None => None
+       end.
+
+  (* Here is where we use the generality of [pointed_Prop], to say
+     that two things of type [var1] are equal, and two things of type
+     [var2] are equal. *)
+  Definition eq_type_and_var : sigT eP -> sigT eP -> option pointed_Prop
+    := fun x y => (eq_semidec_and_gen
+                  base_type_eq_semidec_transparent _ _ var1 (fst (projT2 x)) (fst (projT2 y))
+                /\ eq_semidec_and_gen
+                    base_type_eq_semidec_transparent _ _ var2 (snd (projT2 x)) (snd (projT2 y)))%option_pointed_prop.
+  Definition eq_type_and_const (t t' : flat_type) (x : interp_flat_type t) (y : interp_flat_type t')
+    : option pointed_Prop
+    := eq_semidec_and_gen
+         flat_type_eq_semidec_transparent _ _ interp_flat_type x y.
 
   Definition duplicate_type (ls : list (sigT (fun t => var1 t * var2 t)%type)) : list (sigT eP)
     := List.map (fun v => existT eP (projT1 v, projT1 v) (projT2 v)) ls.
@@ -106,35 +203,21 @@ Section language.
   Lemma duplicate_type_length ls
     : List.length (duplicate_type ls) = List.length ls.
   Proof. apply List.map_length. Qed.
-  (** TODO: Clean up this proof *)
-  Lemma base_type_eq_dec : forall t1 t2 : base_type_code, {t1 = t2} + {t1 <> t2}.
-  Proof.
-    intros t1 t2; destruct (base_type_eq_semidec_transparent t1 t2) eqn:H;
-      [ left; assumption | right; auto using base_type_eq_semidec_is_dec ].
-  Qed.
   Lemma duplicae_type_in t v ls
     : List.In (existT _ (t, t) v) (duplicate_type ls) -> List.In (existT _ t v) ls.
   Proof.
-    unfold duplicate_type; intro H.
-    apply List.in_map_iff in H.
-    destruct H as [ [t' ?] [? ?] ].
-    simpl in *.
-    inversion_sigma; subst.
-    match goal with H : _ |- _ => generalize (path_prod_eta H) end.
-    let x := match goal with |- ?x = _ -> _ => x end in
-    generalize (fst_path x); generalize (snd_path x); simpl.
-    intro; subst; intro H'; intros; subst.
-    assert (H' = eq_refl) by apply UIP_dec, base_type_eq_dec.
-    subst; simpl; assumption.
+    unfold duplicate_type; rewrite List.in_map_iff.
+    intros [ [? ?] [? ?] ].
+    inversion_sigma; inversion_prod; inversion_base_type_code; subst; simpl.
+    assumption.
   Qed.
   Lemma duplicate_type_not_in G t t0 v (H : base_type_eq_semidec_transparent t t0 = None)
     : ~List.In (existT _ (t, t0) v) (duplicate_type G).
   Proof.
     apply base_type_eq_semidec_is_dec in H.
-    clear -H.
-    intro H'.
-    induction G as [|? ? IHG]; simpl in *; try tauto.
-    destruct H'; intuition eauto; congruence.
+    clear -H; intro H'.
+    induction G as [|? ? IHG]; simpl in *; destruct H';
+      intuition; congruence.
   Qed.
 
   Definition preflatten_binding_list2 t1 t2 : option (forall (x : interp_flat_type_gen var1 t1) (y : interp_flat_type_gen var2 t2), list (sigT (fun t => var1 t * var2 t)%type))
@@ -147,6 +230,7 @@ Section language.
        end.
   Definition flatten_binding_list2 t1 t2 : option (forall (x : interp_flat_type_gen var1 t1) (y : interp_flat_type_gen var2 t2), list (sigT eP))
     := option_map (fun f x y => duplicate_type (f x y)) (preflatten_binding_list2 t1 t2).
+  (** This function adds De Bruijn indices to variables *)
   Fixpoint natize_interp_flat_type_gen {var t} (base : nat) (v : interp_flat_type_gen var t) {struct t}
     : nat * interp_flat_type_gen (fun t : base_type_code => nat * var t)%type t
     := match t return interp_flat_type_gen var t -> nat * interp_flat_type_gen _ t with
@@ -174,14 +258,22 @@ Section language.
     rewrite_hyp <- ?*; reflexivity.
   Qed.
 
+  (* This function strips De Bruijn indices from expressions *)
   Fixpoint unnatize_exprf {var t} (base : nat) (e : @exprf (fun t => nat * var t)%type t) : @exprf var t
     := match e in @Syntax.exprf _ _ _ _ t return exprf t with
        | Const _ x => Const x
        | Var _ x => Var (snd x)
        | Op _ _ op args => Op op (@unnatize_exprf _ _ base args)
-       | Let _ ex _ eC => Let (@unnatize_exprf _ _ base ex) (fun x => let v := natize_interp_flat_type_gen base x in
-                                                                  @unnatize_exprf _ _ (fst v) (eC (snd v)))
+       | Let _ ex _ eC => Let (@unnatize_exprf _ _ base ex)
+                             (fun x => let v := natize_interp_flat_type_gen base x in
+                                    @unnatize_exprf _ _ (fst v) (eC (snd v)))
        | Pair _ x _ y => Pair (@unnatize_exprf _ _ base x) (@unnatize_exprf _ _ base y)
+       end.
+  Fixpoint unnatize_expr {var t} (base : nat) (e : @expr (fun t => nat * var t)%type t) : @expr var t
+    := match e in @Syntax.expr _ _ _ _ t return expr t with
+       | Return _ x => unnatize_exprf base x
+       | Abs tx tR f => Abs (fun x : var tx => let v := natize_interp_flat_type_gen (t:=tx) base x in
+                                           @unnatize_expr _ _ (fst v) (f (snd v)))
        end.
 
   Fixpoint reflect_wffT (G : list (sigT (fun t => var1 (fst t) * var2 (snd t))%type))
@@ -204,7 +296,7 @@ Section language.
        | Var _ _, _ => None
        | Op t1 tR op args, Op t1' tR' op' args'
          => match @reflect_wffT G t1 t1' args args', op_beq' t1 tR t1' tR' op op' with
-           | Some p, Some q => Some (p /\ q)
+           | Some p, Some q => Some (p /\ q)%pointed_prop
            | _, _ => None
            end
        | Op _ _ _ _, _ => None
@@ -227,7 +319,31 @@ Section language.
            | _, _ => None
            end
        | Pair _ _ _ _, _ => None
-       end.
+       end%pointed_prop.
+
+    Fixpoint reflect_wfT (G : list (sigT (fun t => var1 (fst t) * var2 (snd t))%type))
+           {t1 t2 : type}
+           (e1 : @expr (fun t => nat * var1 t)%type t1) (e2 : @expr (fun t => nat * var2 t)%type t2)
+           {struct e1}
+    : option pointed_Prop
+    := match e1, e2 return option _ with
+       | Return _ x, Return _ y
+         => reflect_wffT G x y
+       | Return _ _, _ => None
+       | Abs tx tR f, Abs tx' tR' f'
+         => match @flatten_binding_list2 tx tx', type_eq_semidec_transparent tR tR' with
+           | Some G0, Some _
+             => Some (inject (forall (x : interp_flat_type_gen var1 tx) (x' : interp_flat_type_gen var2 tx'),
+                                match @reflect_wfT (G0 x x' ++ G)%list _ _
+                                                   (f (snd (natize_interp_flat_type_gen (List.length G) x)))
+                                                   (f' (snd (natize_interp_flat_type_gen (List.length G) x'))) with
+                                | Some p => to_prop p
+                                | None => False
+                                end))
+           | _, _ => None
+           end
+       | Abs _ _ _, _ => None
+       end%pointed_prop.
 
   Local Ltac handle_op_beq_correct :=
     repeat match goal with
@@ -237,17 +353,22 @@ Section language.
            end.
   Local Ltac t_step :=
     match goal with
-    | _ => progress unfold eq_type_and_var, op_beq', flatten_binding_list2, preflatten_binding_list2, option_map in *
+    | _ => progress unfold eq_type_and_var, op_beq', flatten_binding_list2, preflatten_binding_list2, option_map, and_option_pointed_Prop, eq_semidec_and_gen in *
     | _ => progress simpl in *
     | _ => progress break_match
     | _ => progress subst
     | _ => progress inversion_option
+    | _ => progress inversion_pointed_Prop
     | _ => congruence
     | _ => tauto
     | _ => progress intros
     | _ => progress handle_op_beq_correct
     | _ => progress specialize_by tauto
+    | [ v : sigT _ |- _ ] => destruct v
+    | [ v : prod _ _ |- _ ] => destruct v
     | [ H : forall x x', _ |- wff _ _ _ (flatten_binding_list _ ?x1 ?x2 ++ _)%list _ _ ]
+      => specialize (H x1 x2)
+    | [ H : forall x x', _ |- wf _ _ _ (existT _ _ (?x1, ?x2) :: _)%list _ _ ]
       => specialize (H x1 x2)
     | [ H : and _ _ |- _ ] => destruct H
     | [ H : context[duplicate_type (_ ++ _)%list] |- _ ]
@@ -258,11 +379,14 @@ Section language.
       => rewrite List.app_length in H
     | [ |- wff _ _ _ _ (unnatize_exprf (fst _) _) (unnatize_exprf (fst _) _) ]
       => erewrite length_natize_interp_flat_type_gen1, length_natize_interp_flat_type_gen2; eassumption
+    | [ |- wf _ _ _ _ (unnatize_exprf (fst _) _) (unnatize_exprf (fst _) _) ]
+      => erewrite length_natize_interp_flat_type_gen1, length_natize_interp_flat_type_gen2; eassumption
+    | [ |- @wf _ _ _ _ _ _ (Syntax.Tflat _ _) _ _ ] => constructor
+    | [ |- @wf _ _ _ _ _ _ _ (Syntax.Abs _) (Syntax.Abs _) ] => constructor
     | [ H : base_type_eq_semidec_transparent _ _ = None |- False ] => eapply duplicate_type_not_in; eassumption
     | [ H : List.nth_error _ _ = Some _ |- _ ] => apply List.nth_error_In in H
     | [ H : List.In _ (duplicate_type _) |- _ ] => apply duplicae_type_in in H
     | [ H : context[match _ with _ => _ end] |- _ ] => revert H; progress break_match
-    | [ H : inject _ = inject _ |- _ ] => inversion H; clear H
     | [ |- wff _ _ _ _ _ _ ] => constructor
     | _ => progress unfold and_pointed_Prop in *
     end.
@@ -271,17 +395,15 @@ Section language.
            {t1 t2 : flat_type}
            (e1 : @exprf (fun t => nat * var1 t)%type t1) (e2 : @exprf (fun t => nat * var2 t)%type t2)
            {struct e1}
-    : match reflect_wffT (duplicate_type G) e1 e2 with
-      | Some p => to_prop p
-      | None => False
-      end
-      -> match flat_type_eq_semidec_transparent t1 t2 with
-        | Some p => @wff base_type_code interp_base_type op var1 var2 G t2 (eq_rect _ exprf (unnatize_exprf (List.length G) e1) _ p) (unnatize_exprf (List.length G) e2)
-        | None => False
-        end.
+    : match reflect_wffT (duplicate_type G) e1 e2, flat_type_eq_semidec_transparent t1 t2 with
+      | Some reflective_obligation, Some p
+        => to_prop reflective_obligation
+          -> @wff base_type_code interp_base_type op var1 var2 G t2 (eq_rect _ exprf (unnatize_exprf (List.length G) e1) _ p) (unnatize_exprf (List.length G) e2)
+      | _, _ => True
+      end.
   Proof.
     destruct e1 as [ | | ? ? ? args | tx ex tC eC | ? ex ? ey ],
-                   e2 as [ | | ? ? ? args' | tx' ex' tC' eC' | ? ex' ? ey' ]; simpl; try solve [ intros [] ];
+                   e2 as [ | | ? ? ? args' | tx' ex' tC' eC' | ? ex' ? ey' ]; simpl; try solve [ exact I ];
       [ clear reflect_wff
       | clear reflect_wff
       | specialize (reflect_wff G _ _ args args')
@@ -303,4 +425,82 @@ Section language.
     { t. }
     { t. }
   Qed.
+  Fixpoint reflect_wf (G : list (sigT (fun t => var1 t * var2 t)%type))
+           {t1 t2 : type}
+           (e1 : @expr (fun t => nat * var1 t)%type t1) (e2 : @expr (fun t => nat * var2 t)%type t2)
+    : match reflect_wfT (duplicate_type G) e1 e2, type_eq_semidec_transparent t1 t2 with
+      | Some reflective_obligation, Some p
+        => to_prop reflective_obligation
+          -> @wf base_type_code interp_base_type op var1 var2 G t2 (eq_rect _ expr (unnatize_expr (List.length G) e1) _ p) (unnatize_expr (List.length G) e2)
+      | _, _ => True
+      end.
+  Proof.
+    destruct e1 as [ t1 e1 | tx tR f ],
+                   e2 as [ t2 e2 | tx' tR' f' ]; simpl; try solve [ exact I ];
+      [ clear reflect_wf;
+        pose proof (@reflect_wff G t1 t2 e1 e2)
+      | pose proof (fun x x'
+                    => match preflatten_binding_list2 tx tx' as v return match v with Some _ => _ | None => True end with
+                      | Some G0
+                        => reflect_wf
+                            (G0 x x' ++ G)%list _ _
+                            (f (snd (natize_interp_flat_type_gen (length (duplicate_type G)) x)))
+                            (f' (snd (natize_interp_flat_type_gen (length (duplicate_type G)) x')))
+                      | None => I
+                      end);
+        clear reflect_wf ].
+    { t. }
+    { t. }
+  Qed.
 End language.
+
+Section Wf.
+  Context (base_type_code : Type)
+          (interp_base_type : base_type_code -> Type)
+          (base_type_eq_semidec_transparent : forall t1 t2 : base_type_code, option (t1 = t2))
+          (base_type_eq_semidec_is_dec : forall t1 t2, base_type_eq_semidec_transparent t1 t2 = None -> t1 <> t2)
+          (op : flat_type base_type_code -> flat_type base_type_code -> Type)
+          (op_beq : forall t1 tR, op t1 tR -> op t1 tR -> option pointed_Prop)
+          (op_beq_bl : forall t1 tR x y, prop_of_option (op_beq t1 tR x y) -> x = y)
+          {t : type base_type_code}
+          (e : @Expr base_type_code interp_base_type op t).
+
+  (** Leads to smaller proofs, but is less generally applicable *)
+  Theorem reflect_Wf_unnatize
+    : (forall var1 var2,
+          prop_of_option (@reflect_wfT base_type_code interp_base_type base_type_eq_semidec_transparent op op_beq var1 var2 nil t t (e _) (e _)))
+      -> Wf _ _ _ (fun var => unnatize_expr base_type_code interp_base_type op 0 (e (fun t => (nat * var t)%type))).
+  Proof.
+    intros H var1 var2; specialize (H var1 var2).
+    pose proof (@reflect_wf base_type_code interp_base_type base_type_eq_semidec_transparent base_type_eq_semidec_is_dec op op_beq op_beq_bl var1 var2 nil t t (e _) (e _)) as H'.
+    rewrite type_eq_semidec_transparent_refl in H' by assumption.
+    edestruct reflect_wfT; simpl in *; tauto.
+  Qed.
+
+  (** Leads to larger proofs (an extra constant factor which is the
+      size of the expression tree), but more generally applicable *)
+  Theorem reflect_Wf
+    : (forall var1 var2,
+          unnatize_expr base_type_code interp_base_type op 0 (e (fun t => (nat * var1 t)%type)) = e _
+          /\ prop_of_option (@reflect_wfT base_type_code interp_base_type base_type_eq_semidec_transparent op op_beq var1 var2 nil t t (e _) (e _)))
+      -> Wf _ _ _ e.
+  Proof.
+    intros H var1 var2.
+    rewrite <- (proj1 (H var1 var2)), <- (proj1 (H var2 var2)).
+    apply reflect_Wf_unnatize, H.
+  Qed.
+End Wf.
+
+
+Ltac generalize_reflect_Wf base_type_eq_semidec_is_dec op_beq_bl :=
+  lazymatch goal with
+  | [ |- @Wf ?base_type_code ?interp_base_type ?op ?t ?e ]
+    => generalize (@reflect_Wf_unnatize base_type_code interp_base_type _ base_type_eq_semidec_is_dec op _ op_beq_bl t e)
+  end.
+Ltac use_reflect_Wf := vm_compute; let H := fresh in intro H; apply H; clear H.
+Ltac fin_reflect_Wf := repeat constructor.
+(** The tactic [reflect_Wf] is the main tactic of this file, used to
+    prove [Syntax.Wf] goals *)
+Ltac reflect_Wf base_type_eq_semidec_is_dec op_beq_bl :=
+  generalize_reflect_Wf base_type_eq_semidec_is_dec op_beq_bl;
+  use_reflect_Wf; fin_reflect_Wf.
